code/ecdsap256/Hacl.P256.fst
@@ -45,7 +45,7 @@ let ecdsa_verif_without_hash mLen m pubKey r s  =
 
 
 let validate_public_key pubKey =
-  Hacl.Impl.P256.Point.verifyQ pubKey
+  Hacl.Impl.P256.Point.validate_pubkey pubKey
 
 let validate_private_key x =
   Hacl.Impl.P256.Point.isMoreThanZeroLessThanOrder x
